Rope/WF.lean
@@ -6,33 +6,39 @@ public import Rope.Label
 
 namespace WF
 
-open Pre Label WF
-
+open Label
 
 -- Interdefined Well-formedness rules for Pre.Row and Pre.Ty
 mutual
-inductive WF_Ty : (inner: Pre.Row) -> Prop where
-  | empty : WF_Ty .empty
-  | rVar : WF_Ty (.rVar s)
-  | extend : WF_Ty r -> Pre.Row.unique_labels r -> r.lack l -> (WF_Row t) -> WF_Ty (.extend r l t)
+inductive WF_Row : (inner: Pre.Row) -> Prop where
+  | empty : WF_Row .empty
+  | rVar : WF_Row (.rVar s)
+  | extend : WF_Row r -> r.lack l -> (WF_Ty t) -> WF_Row (.extend r l t)
 
-inductive WF_Row : (inner: Pre.Ty) -> Prop where
-  | TVar : WF_Row (.TVar s)
-  | TFun : WF_Row arg -> WF_Row ret -> WF_Row (.TFun (arg: Pre.Ty) (ret: Pre.Ty))
-  | Singleton : WF_Row (.Singleton l)
-  | Pi : WF_Ty r -> WF_Row (.Pi r)
-  | Sigma : WF_Ty r -> WF_Row (.Sigma r)
+inductive WF_Ty : (inner: Pre.Ty) -> Prop where
+  | TVar : WF_Ty (.TVar s)
+  | TFun : WF_Ty arg -> WF_Ty ret -> WF_Ty (.TFun (arg: Pre.Ty) (ret: Pre.Ty))
+  | Singleton : WF_Ty (.Singleton l)
+  | Pi : WF_Row r -> WF_Ty (.Pi r)
+  | Sigma : WF_Row r -> WF_Ty (.Sigma r)
 end
+
+theorem WF.unique_labels {r : Pre.Row} (wf : WF_Row r) : r.unique_labels :=
+  match wf with
+  | .empty => .empty
+  | .rVar => .rVar
+  | .extend r_wf r_lack_l ty_wf => Pre.Row.unique_labels.extend (WF.unique_labels r_wf) r_lack_l
 
 -- TODO set up wellfounded induction over Rows and Tys
 structure Row : Type where
   inner : Pre.Row
-  wf : WF_Ty inner
+  wf : WF_Row inner
 -- Row must be implemented on top of Pre.Row and bundle well-formedness invariant
 
 structure Ty : Type where
   inner : Pre.Ty
-  wf : WF_Row inner
+  wf : WF_Ty inner
+
 
 def Row.unique_labels : Row -> Prop
   | .mk inner _ => inner.unique_labels
@@ -41,98 +47,230 @@ def Row.unique_labels : Row -> Prop
 def Row.lack : Row -> Label -> Prop
   | ⟨inner, _⟩, l => inner.lack l
 
-def Row.has_label : Row -> Label -> Prop
-  | ⟨inner, _⟩, l => inner.has_label l
-
 def Row.disjoint : Row -> Row -> Prop
   | ⟨innerL, _⟩, ⟨innerR, _⟩ => innerL.disjoint innerR
 
 def Row.concrete : Row -> Prop
   | ⟨inner, _⟩ => inner.concrete
 
+@[match_pattern]
+def Row.empty : Row := ⟨.empty, .empty⟩
 
-def Row.type_at_helper (r : Pre.Row) (l : Label) (h : WF_Ty r): Option Ty :=
+@[match_pattern]
+def Row.extend (r: Row) (l : Label) (t : Ty) (h: r.lack l) : Row  :=
+    ⟨Pre.Row.extend r.inner l t.inner, .extend r.wf h t.wf⟩
+
+def Row.rVar (name : String) : Row :=
+  ⟨.rVar name, .rVar⟩
+
+-- @[match_pattern]
+-- def Ty.TFun (t1 t2 : Ty) : Ty :=
+--   ⟨Pre.Ty.TFun t1.inner t2.inner, WF_Ty.TFun t1.wf t2.wf⟩
+
+-- @[match_pattern]
+-- def Ty.Singleton (l : Label) : Ty :=
+--   {
+--     inner := Pre.Ty.Singleton l,
+--     wf := WF_Ty.Singleton
+--   }
+
+-- @[match_pattern]
+-- def Ty.Pi (r : Row) : Ty :=
+--   {
+--     inner := Pre.Ty.Pi r.inner,
+--     wf := WF_Ty.Pi r.wf
+--   }
+
+-- @[match_pattern]
+-- def Ty.Sigma (r : Row) : Ty :=
+--   {
+--     inner := Pre.Ty.Sigma r.inner,
+--     wf := WF_Ty.Sigma r.wf
+--   }
+
+-- inductive Row.has_label : Row -> Label -> Prop where
+--   | first {r l t} : (h : r.lack l) -> has_label (.extend r l t h) l
+--   | extend {r l l' t} : (h : r.lack l') -> r.has_label l -> has_label (.extend r l' t h) l
+
+def Row.has_label (r : Row) (l : Label): Prop :=
+  r.inner.has_label l
+
+
+def Row.type_at (r : Row) (l : Label): Option Ty :=
   match r with
-  | .empty => .none
-  | .rVar _ => .none
-  | .extend r' l' t =>
+  | ⟨.empty, _⟩ => .none
+  | ⟨.rVar _, _⟩ => .none
+  | ⟨.extend r' l' t, wf⟩ =>
      if l = l'
-      then .some {inner := t, wf := (by cases h ; assumption)}
-      else type_at_helper r' l (by cases h ; assumption)
+      then .some ⟨t, (match wf with | .extend _ _ wft => wft)⟩
+      else type_at ⟨r', (match wf with | .extend wfr _ _ => wfr)⟩ l
 
-def Row.type_at : Row -> Label -> Option Ty
-  | ⟨inner, wf⟩, l => type_at_helper inner l wf
+theorem Row.type_at_is_some {r : Row} {l: Label} (h : r.has_label l) : (Option.isSome (r.type_at l) = true) :=
+  match r with
+  | ⟨inner, wf⟩ =>
+    match inner with
+    | .empty => by contradiction
+    | .extend r' l' t' =>
+      -- match h with
+      -- | @Row.has_label.first _ _ _ _  => by
+      --   simp [type_at]
+      -- | @Row.has_label.extend r' l1' l2' t h_lack has_l =>
+      --   dite (l1' = l2')
+      --   (λ h => by
+      --     simp [Row.type_at,h]
+      --     )
+      --   (λ h => by
+      --     simp [Row.type_at, h]
+      --     apply Row.type_at_is_some has_l)
+        by
+          by_cases (l = l')
+          case _ h_pos => simp [type_at, h_pos]
+          case _ h_neg =>
+            cases h;
+            contradiction
+            simp [type_at, h_neg]
+            case extend h =>
+              apply Row.type_at_is_some
+              simp [has_label,h]
+          -- apply Row.type_at_is_some
+    
+def Row.type_at! (r: Row) (l: Label) (has_l : has_label r l) : Ty :=
+  (r.type_at l).get (Row.type_at_is_some has_l)
+  
 
-
-def Row.le (a b : Row) : Prop :=
-  a.inner.le b.inner
+-- def Row.le (a b : Row) : Prop :=
+--   a.inner.le b.inner
 
 theorem lacks_extend_lacks {r: Pre.Row} {l1 l2: Label} {t: Pre.Ty} (h_lack: Pre.Row.lack (r.extend l2 t) l1) : Pre.Row.lack r l1 :=
   match h_lack with
   | .extend h' _ => h'
 
-instance : LE Row where
-  le := Row.le
 
-theorem Row.le_inner_has_label {r1 r2 : Row} {l : Label } (h_le : r1 ≤ r2) (h_has : r2.inner.has_label l) : r1.inner.has_label l := by
-  simp [(.≤.), Row.le, Pre.Row.le] at h_le
-  apply (h_le _ h_has).left
 
-theorem Row.le_trans (r1 r2 r3 : Row) (h_1_2 : r1 ≤ r2) (h_2_3 : r2 ≤ r3) : r1 ≤ r3 :=
-  λ l h => by
-    apply And.intro
-    case left =>
-      apply le_inner_has_label h_1_2 (le_inner_has_label h_2_3 h)
-    case right =>
-      simp [(.≤.),Row.le,Pre.Row.le] at *
-      grind
-
-theorem Row.le_refl : ∀ (x : Row), x ≤ x :=
-  λ _ _ h => And.intro h rfl
-
-instance : Std.IsPreorder Row where
-  le_refl := Row.le_refl
-  le_trans := Row.le_trans
-
+@[match_pattern]
 def Ty.TVar (s : String) : Ty :=
-  ⟨Pre.Ty.TVar s, WF_Row.TVar⟩
+  ⟨Pre.Ty.TVar s, WF_Ty.TVar⟩
 
+@[match_pattern]
 def Ty.TFun (t1 t2 : Ty) : Ty :=
-  ⟨Pre.Ty.TFun t1.inner t2.inner, WF_Row.TFun t1.wf t2.wf⟩
+  ⟨Pre.Ty.TFun t1.inner t2.inner, WF_Ty.TFun t1.wf t2.wf⟩
 
+@[match_pattern]
 def Ty.Singleton (l : Label) : Ty :=
   {
     inner := Pre.Ty.Singleton l,
-    wf := WF_Row.Singleton
+    wf := WF_Ty.Singleton
   }
 
+@[match_pattern]
 def Ty.Pi (r : Row) : Ty :=
   {
     inner := Pre.Ty.Pi r.inner,
-    wf := WF_Row.Pi r.wf
+    wf := WF_Ty.Pi r.wf
   }
 
+@[match_pattern]
 def Ty.Sigma (r : Row) : Ty :=
   {
     inner := Pre.Ty.Sigma r.inner,
-    wf := WF_Row.Sigma r.wf
+    wf := WF_Ty.Sigma r.wf
   }
 
+-- def get_helper : r.has_label l -> Option.isSome (type_at r l) := sorry
+
+-- def le2_helper (e: Ty -> Ty -> Prop) (l : Label) (a b : Row) : Prop :=
+--   (b.has_label l -> a.has_label l) ∧
+--     (((a.has_label l ∧ b.has_label l )) -> e ((type_at a l).get) ((type_at b l).get (get_helper h.right)))
 
 mutual
+-- inductive option_equiv  : Option Ty -> Option Ty -> Prop where
+--   | none : option_equiv .none .none 
+--   | some : (Ty.Equiv t1 t2) -> option_equiv (.some t1) (.some t2)
+inductive Row.le : Row -> Row -> Prop where
+  | empty {r : Row} : Row.le .empty r
+  | rVar {name : String} : Row.le (.rVar name) (.rVar name)
+  | extend {a b : Row} {l : Label} {t : Ty} :
+    Row.le a b -> (h_lack : a.lack l) -> b.has_label l -> Row.le (@a.extend l t h_lack) b
+-- | empty : Row.le2 Row.empty Row.empty
+-- | head : Row.le2
+-- | mk {a b : Row} : forall l, (a.has_label l -> b.has_label l) -> () -> Row.le a b
+
+-- Alternate definition for le. Requires 1 less assumption in the extend case, but doesn't match our induction structure as well
+inductive Row.le2 : Row -> Row -> Prop where
+  | refl {r : Row} : Row.le2 r r
+  | extendR {a b : Row} {l : Label} {t : Ty} : (h_lack : b.lack l) -> Row.le2 a b -> Row.le2 a (b.extend l t h_lack)
+  | extend2 {a b : Row} {l : Label} {ta tb : Ty} :
+    Row.le2 a b -> (ha_lack : a.lack l) -> (hb_lack : b.lack l) -> Ty.Equiv ta tb -> Row.le2 (a.extend l ta ha_lack) (b.extend l tb hb_lack)
+-- def Row.le (a b: Row) : Prop :=
+  -- forall (l : Label), b.inner.has_label l -> a.inner.has_label l ∧ (type_at a l) = (type_at b l)
 
 inductive Ty.Equiv : Ty  -> Ty  -> Prop where
   | TVar : Ty.Equiv (Ty.TVar s) (Ty.TVar s)
   | Singleton : Ty.Equiv (Ty.Singleton l) (Ty.Singleton l)
-  | Pi : Row.Equiv r1 r2 -> Ty.Equiv (Ty.Pi r1) (Ty.Pi r2)
-  | Sigma : Row.Equiv r1 r2 -> Ty.Equiv (Ty.Sigma r1) (Ty.Sigma r2)
+  | Pi : a.le b -> b.le a -> Ty.Equiv (Ty.Pi a) (Ty.Pi b)
+  | Sigma : a.le b -> b.le a -> Ty.Equiv (Ty.Sigma a) (Ty.Sigma b)
   | TFun : Ty.Equiv a1 a2 -> Ty.Equiv r1 r2 -> Ty.Equiv (Ty.TFun a1 r1) (Ty.TFun a2 r2)
-
-inductive Row.Equiv : Row  -> Row  -> Prop where
-  | mk {a b : Row} : a ≤ b ∧ b ≤ a -> Row.Equiv a b
 end
 
-theorem Row.Equiv.refl : ∀ r: Row, r.Equiv r :=
+inductive Row.Equiv : WF.Row -> WF.Row  -> Prop where
+  | mk {a b : WF.Row} : Row.le a b ∧ Row.le b a -> Row.Equiv a b
+
+-- Ideas for deciding le and equiv
+-- sort row and compare in order
+-- convert row to a hashmap
+-- Redefine a WF row to always be sorted, then define le inductively over the sorted row
+
+instance : LE Row where
+  le := Row.le
+
+def Row.ble (a b : Row) : Bool := sorry
+
+-- theorem Row.ble_decides_le : ∀ r1 r2: Row, r1.ble r2 = true <-> r1 ≤ r2 := by sorry
+
+-- instance : DecidableLE Row := by
+--   intro a b
+--   by_cases a.ble b
+--   case pos h =>
+--     apply Decidable.isTrue
+--     exact (Row.ble_decides_le a b).mp h
+--   case neg h =>
+--     sorry
+
+theorem Row.le_inner_has_label {a b : Row} {l : Label } (h_le : a ≤ b) (h_has : a.inner.has_label l) : b.inner.has_label l :=
+    match h_le with
+    | .empty => by contradiction
+    | @Row.le.extend a' _ l' _ a'_le_b a'_lack_l' b_has_l' =>
+        dite (l = l')
+        (λ hpos => by
+          simp [hpos, Row.has_label,Row.extend] at *;
+          exact b_has_l')
+        (λ hneg =>
+          match h_has with
+          | .first => b_has_l'
+          | .extend h => @Row.le_inner_has_label a' b _ a'_le_b h)
+
+theorem Row.le_trans (a b c : Row) (h_a_b : a ≤ b) (h_b_c : b ≤ c) : a ≤ c :=
+  match h_a_b with
+  | .empty => .empty
+  | .rVar => sorry
+  | .extend a'_le_b h_lack h_lab =>
+    .extend (le_trans _ _ _ a'_le_b h_b_c) _ (Row.le_inner_has_label h_b_c h_lab)
+  -- by exact le_inner_has_label h_a_b (le_inner_has_label _ _)
+
+  --   case right =>
+  --     simp [(.≤.),Row.le] at *
+  --     grind
+
+theorem Row.le_refl : ∀ (x : Row), x ≤ x :=
+  λ x =>
+  match x with
+  | Row.empty => .empty
+  | .rVar _ => .rVar
+  | ⟨Pre.Row.extend r _ _, .extend _ _ _⟩ => sorry
+
+instance : Std.IsPreorder Row := ⟨Row.le_refl, Row.le_trans⟩
+
+theorem Row.Equiv.refl : ∀ (r: Row), r.Equiv r :=
   λ _ => .mk (And.intro
           (instIsPreorderRow.le_refl _)
           (instIsPreorderRow.le_refl _))
@@ -147,20 +285,21 @@ theorem Row.Equiv.trans : ∀ {x y z: Row}, x.Equiv y → y.Equiv z → x.Equiv 
   apply Equiv.mk
   apply And.intro <;>
     cases h_x_y <;> cases h_y_z <;>
-    simp [.≤.,Row.le,Pre.Row.le] at * <;>
-    grind
+    -- simp [.≤.,Row.le] at * <;>
+    -- grind
+    sorry
 
-theorem Ty.Equiv.refl : ∀ x, Ty.Equiv x x :=
+theorem Ty.Equiv.refl : ∀ x : Ty, Ty.Equiv x x :=
   λ x =>
       match x with
       | .TVar _ => .TVar
       | .Singleton _ => .Singleton
-      | ⟨.TFun arg ret, WF_Row.TFun wf_a wf_r⟩ =>
+      | ⟨.TFun arg ret, WF_Ty.TFun wf_a wf_r⟩ =>
         @Equiv.TFun ⟨arg,wf_a⟩ ⟨arg,wf_a⟩ ⟨ret, wf_r⟩ ⟨ret, wf_r⟩ (.refl _) (.refl _)
-      | ⟨.Pi r, WF_Row.Pi wf_r⟩ =>
-        @Equiv.Pi ⟨r, wf_r⟩ ⟨r, wf_r⟩ (Row.Equiv.refl _)
-      | ⟨.Sigma r, WF_Row.Sigma wf_r⟩ =>
-        @Equiv.Sigma ⟨r, wf_r⟩ ⟨r, wf_r⟩ (Row.Equiv.refl _)
+      | ⟨.Pi r, WF_Ty.Pi wf_r⟩ =>
+        @Equiv.Pi ⟨r, wf_r⟩ ⟨r, wf_r⟩ (Row.le_refl _) (Row.le_refl _)
+      | ⟨.Sigma r, WF_Ty.Sigma wf_r⟩ =>
+        @Equiv.Sigma ⟨r, wf_r⟩ ⟨r, wf_r⟩ (Row.le_refl _) (Row.le_refl _)
 
 theorem Ty.Equiv.symm : ∀ {x y : Ty}, x.Equiv y → y.Equiv x :=
   λ h =>
@@ -168,8 +307,8 @@ theorem Ty.Equiv.symm : ∀ {x y : Ty}, x.Equiv y → y.Equiv x :=
     | .TVar => Ty.Equiv.TVar
     | .Singleton => .Singleton
     | .TFun h1 h2 => .TFun (Ty.Equiv.symm h1) (Ty.Equiv.symm h2)
-    | .Pi h => .Pi (Row.Equiv.symm h)
-    | .Sigma h => .Sigma (Row.Equiv.symm h)
+    | .Pi hl hr => .Pi hr hl
+    | .Sigma hl hr => .Sigma hr hl
 
 theorem Ty.Equiv.trans : ∀ {x y z : Ty}, x.Equiv y → y.Equiv z → x.Equiv z :=
   @λ x y z h1 h2 =>
@@ -184,10 +323,10 @@ theorem Ty.Equiv.trans : ∀ {x y z : Ty}, x.Equiv y → y.Equiv z → x.Equiv z
           Equiv.TFun (Ty.Equiv.trans h1a h2a) (Ty.Equiv.trans h1r h2r)
     | ⟨.Pi _, _⟩, _, _ =>
       match h1, h2 with
-      | @Equiv.Pi _ ⟨_, _⟩ h_xy, Equiv.Pi h_yz => Ty.Equiv.Pi (Row.Equiv.trans h_xy h_yz)
+      | @Equiv.Pi _ ⟨_, _⟩ h_xy h_yx, Equiv.Pi h_yz h_zy => Ty.Equiv.Pi (Row.le_trans _ _ _ h_xy h_yz) (Row.le_trans _ _ _ h_zy h_yx)
     | ⟨.Sigma _, _⟩, _, _ =>
       match h1, h2 with
-      | @Equiv.Sigma _ ⟨_, _⟩ h_xy, Equiv.Sigma h_yz => Ty.Equiv.Sigma (Row.Equiv.trans h_xy h_yz)
+      | @Equiv.Sigma _ ⟨_, _⟩ h_xy h_yx, Equiv.Sigma h_yz h_zy => Ty.Equiv.Sigma (Row.le_trans _ _ _ h_xy h_yz) (Row.le_trans _ _ _ h_zy h_yx)
 
 -- This definition of equivalence is syntactic, up to reordering of fields
 -- Equivalence of rows with respect to a context or substitution will be defined over quotients of well-formed rows and types
