Rope/Basic.lean
@@ -4,8 +4,26 @@ public import Rope.WF
 
 @[expose] public section
 
+-- open WF
+
+
 def Row : Type := Quotient WF.Row.instSetoid
 
 def Ty : Type := Quotient WF.Ty.instSetoid
 
-end
+instance : LE Row where
+  le :=
+    Quotient.lift₂ WF.Row.le <| by
+      intro a1 b1 a2 b2 aeq beq
+      cases aeq; cases beq;
+      case _ ha hb =>
+        
+        
+        sorry
+
+-- def lack (r1 r2 : Row) : Prop :=
+--   Quotient.lift WF.lack <| by
+--     sorry
+--     sorry
+--     sorry
+
